coq/thielemachine/coqproofs/SpacelandComplete.v
@@ -146,8 +146,11 @@ Module Dynamics.
       destruct t2 as [s2' | s2' l2 t2']; simpl in *.
       + (* t2 = TNil *)
         simpl in Hi1. simpl in Hi2.
-        subst.
-        split; reflexivity.
+        split.
+        * (* partition_seq *)
+          simpl. f_equal. rewrite Hi1, Hi2. simpl. reflexivity.
+        * (* mu_seq *)
+          simpl. reflexivity.
       + (* t2 = TCons *) discriminate.
     - (* t1 = TCons *)
       destruct t2 as [s2' | s2' l2 t2']; simpl in *.
